RocqOfRust/core/simulate/option.v
@@ -1,8 +1,49 @@
 Require Import simulate.RocqOfRust.
 Require Import core.links.option.
+Require Import core.simulate.default.
 
 Module Impl_Option.
   Definition Self (T : Set) : Set := option T.
+
+  Lemma unwrap_eq {T : Set} `{Link T} (stack : Stack.t) (self : Self T) (value : T) :
+    self = Some value ->
+    {{
+      SimulateM.eval_f (Impl_Option.run_unwrap self) stack 🌲
+      (Output.Success value, stack)
+    }}.
+  Proof.
+    intros.
+    subst.
+    s.
+  Qed.
+
+  Definition unwrap_or_default
+      {T : Set} `{Default.C T}
+      (self : Self T) : T :=
+    match self with
+    | Some value => value
+    | None => Default.default
+    end.
+
+  Lemma unwrap_or_default_eq
+      {T : Set} `{Link T}
+      `{!default.Default.Run T}
+      `{Default_for_T : Default.C T}
+      `{!Default.Eq.C (Self := T) Default_for_T}
+      (stack : Stack.t) (self : Self T) :
+    {{
+      SimulateM.eval_f (Impl_Option.run_unwrap_or_default self) stack 🌲
+      (Output.Success (unwrap_or_default self), stack)
+    }}.
+  Proof.
+    destruct self; cbn.
+    { s. }
+    { s. {
+        apply Default.Eq.default.
+      }
+      s.
+    }
+  Qed.
 
   (* pub fn unwrap_or(self, default: T) -> T *)
   Definition unwrap_or {T : Set} (self : Self T) (default : T) : T :=
@@ -22,5 +63,7 @@ Module Impl_Option.
         stack
       )
     }}.
-  Admitted.
+  Proof.
+    destruct self; s.
+  Qed.
 End Impl_Option.
