RocqOfRust/revm/revm_interpreter/instructions/simulate/utility.v
@@ -3,6 +3,7 @@ Require Import alloy_primitives.bits.links.address.
 Require Import alloy_primitives.bits.simulate.address.
 Require Import alloy_primitives.bits.simulate.fixed.
 Require Import alloy_primitives.links.aliases.
+Require Import core.convert.simulate.mod.
 Require Import revm.revm_interpreter.instructions.links.utility.
 Require Import ruint.links.lib.
 
@@ -33,6 +34,122 @@ Lemma cast_slice_to_address_like
   end.
 Admitted.
 
+Module IntoU256.
+  Class C (Self : Set) : Set := {
+    into_u256 (self : Self) : aliases.U256.t;
+  }.
+
+  Module Eq.
+    Class C
+        {Self : Set} `{Link Self}
+        `{!utility.IntoU256.Run Self}
+        `(!IntoU256.C Self) :
+        Prop := {
+      into_u256 (self : Self) (stack : Stack.t) :
+        {{
+          SimulateM.eval_f
+            (utility.IntoU256.run_into_u256 self)
+            stack 🌲
+          (
+            Output.Success (into_u256 self),
+            stack
+          )
+        }};
+    }.
+  End Eq.
+  Export (hints) Eq.
+End IntoU256.
+Export (hints) IntoU256.
+
+Module Impl_IntoU256_for_B256.
+  Definition Self : Set :=
+    aliases.B256.t.
+
+  Definition into_u256 (self : Self) : aliases.U256.t :=
+    Impl_From_FixedBytes_32_for_U256.from self.
+
+  Lemma into_u256_eq (self : Self) (stack : Stack.t) :
+    {{
+      SimulateM.eval_f
+        (utility.Impl_IntoU256_for_B256.run_into_u256 self)
+        stack 🌲
+      (Output.Success (into_u256 self), stack)
+    }}.
+  Admitted.
+
+  Instance I : IntoU256.C Self := {|
+    IntoU256.into_u256 := into_u256;
+  |}.
+
+  Module Eq.
+    Instance I : IntoU256.Eq.C (Self := Self) Impl_IntoU256_for_B256.I.
+    Proof.
+      constructor.
+      apply into_u256_eq.
+    Qed.
+  End Eq.
+  Export (hints) Eq.
+End Impl_IntoU256_for_B256.
+Export (hints) Impl_IntoU256_for_B256.
+
+Module Impl_IntoU256_for_Address.
+  Definition Self : Set :=
+    Address.t.
+
+  Definition into_u256 (self : Self) : aliases.U256.t :=
+    Impl_From_FixedBytes_32_for_U256.from (Impl_Address.into_word self).
+
+  Lemma into_u256_eq (self : Self) (stack : Stack.t) :
+    {{
+      SimulateM.eval_f
+        (utility.Impl_IntoU256_for_Address.run_into_u256 self)
+        stack 🌲
+      (Output.Success (into_u256 self), stack)
+    }}.
+  Admitted.
+
+  Instance I : IntoU256.C Self := {|
+    IntoU256.into_u256 := into_u256;
+  |}.
+
+  Module Eq.
+    Instance I : IntoU256.Eq.C (Self := Self) Impl_IntoU256_for_Address.I.
+    Proof.
+      constructor.
+      apply into_u256_eq.
+    Qed.
+  End Eq.
+  Export (hints) Eq.
+End Impl_IntoU256_for_Address.
+Export (hints) Impl_IntoU256_for_Address.
+
+Module IntoAddress.
+  Class C (Self : Set) : Set := {
+    into_address (self : Self) : Address.t;
+  }.
+
+  Module Eq.
+    Class C
+        {Self : Set} `{Link Self}
+        `{!utility.IntoAddress.Run Self}
+        `(!IntoAddress.C Self) :
+        Prop := {
+      into_address (self : Self) (stack : Stack.t) :
+        {{
+          SimulateM.eval_f
+            (utility.IntoAddress.run_into_address self)
+            stack 🌲
+          (
+            Output.Success (into_address self),
+            stack
+          )
+        }};
+    }.
+  End Eq.
+  Export (hints) Eq.
+End IntoAddress.
+Export (hints) IntoAddress.
+
 Module Impl_IntoAddress_for_U256.
   Definition into_address (self : aliases.U256.t) : Address.t :=
     Impl_Address.from_word (Impl_From_U256_for_FixedBytes_32.from self).
@@ -46,4 +163,18 @@ Module Impl_IntoAddress_for_U256.
     }}.
   Proof.
   Admitted.
+
+  Instance I : IntoAddress.C aliases.U256.t := {|
+    IntoAddress.into_address := into_address;
+  |}.
+
+  Module Eq.
+    Instance I : IntoAddress.Eq.C (Self := aliases.U256.t) Impl_IntoAddress_for_U256.I.
+    Proof.
+      constructor.
+      apply into_address_eq.
+    Qed.
+  End Eq.
+  Export (hints) Eq.
 End Impl_IntoAddress_for_U256.
+Export (hints) Impl_IntoAddress_for_U256.
