RocqOfRust/revm/revm_interpreter/instructions/tests/contract.v
@@ -1,5 +1,8 @@
 Require Import simulate.RocqOfRust.
 Require Import alloy_primitives.bits.links.address.
+Require Import alloy_primitives.bytes.links.mod.
+Require Import alloy_primitives.links.aliases.
+Require Import alloy_primitives.log.links.mod.
 Require Import revm.revm_context_interface.links.host.
 Require Import revm.revm_context_interface.links.journaled_state.
 Require Import revm.revm_context_interface.simulate.host.
@@ -9,6 +12,7 @@ Require Import revm.revm_interpreter.links.instruction_result.
 Require Import revm.revm_interpreter.tests.interpreter.
 Require Import revm.revm_interpreter.tests.interpreter_types.
 Require Import ruint.links.lib.
+Require Import ruint.simulate.lib.
 
 (** Mock Host that returns None - for FatalExternalError path *)
 Module TestHost.
@@ -17,12 +21,128 @@ Module TestHost.
   Instance IsLink : Link t.
   Admitted.
 
+  Definition cfg : RefStub.t t t := {|
+    RefStub.path := [];
+    RefStub.projection self := self;
+    RefStub.injection _ y := y;
+  |}.
+  Definition block : RefStub.t t t := {|
+    RefStub.path := [];
+    RefStub.projection self := self;
+    RefStub.injection _ y := y;
+  |}.
+
+  Definition chain_id (_self : t) : u64 := {| Integer.value := 1 |}.
+  Definition spec (_self : t) : t := Make.
+  Definition max_code_size (_self : t) : usize := {| Integer.value := 0 |}.
+  Definition is_eip3607_disabled (_self : t) : bool := false.
+  Definition is_balance_check_disabled (_self : t) : bool := false.
+  Definition is_gas_refund_disabled (_self : t) : bool := false.
+  Definition is_block_gas_limit_disabled (_self : t) : bool := false.
+  Definition is_nonce_check_disabled (_self : t) : bool := false.
+  Definition is_base_fee_check_disabled (_self : t) : bool := false.
+  Definition number (_self : t) : u64 := {| Integer.value := 1 |}.
+  Definition beneficiary (_self : t) : Address.t := {| Address.value := 0 |}.
+  Definition timestamp (_self : t) : u64 := {| Integer.value := 0 |}.
+  Definition gas_limit (_self : t) : u64 := {| Integer.value := 0 |}.
+  Definition basefee (_self : t) : u64 := {| Integer.value := 0 |}.
+  Definition difficulty (_self : t) : aliases.U256.t := Impl_Uint.ZERO.
+  Definition prevrandao (_self : t) : option aliases.B256.t := None.
+  Definition blob_gasprice (_self : t) : option u128 := None.
+
   Definition load_account_delegated (self : t) (address : Address.t) :
       option AccountLoad.t * t :=
     (None, Make).
 
+  Definition block_hash (self : t) (_number : u64) :
+      option aliases.B256.t * t :=
+    (None, Make).
+
+  Definition balance (self : t) (_address : Address.t) :
+      option (StateLoad.t aliases.U256.t) * t :=
+    (None, Make).
+
+  Definition code (self : t) (_address : Address.t) :
+      option (Eip7702CodeLoad.t Bytes.t) * t :=
+    (None, Make).
+
+  Definition code_hash (self : t) (_address : Address.t) :
+      option (Eip7702CodeLoad.t aliases.B256.t) * t :=
+    (None, Make).
+
+  Definition sload (self : t) (_address : Address.t) (_index : aliases.U256.t) :
+      option (StateLoad.t aliases.U256.t) * t :=
+    (None, Make).
+
+  Definition sstore
+      (self : t)
+      (_address : Address.t)
+      (_index : aliases.U256.t)
+      (_value : aliases.U256.t) :
+      option (StateLoad.t SStoreResult.t) * t :=
+    (None, Make).
+
+  Definition tload (self : t) (_address : Address.t) (_index : aliases.U256.t) :
+      aliases.U256.t * t :=
+    (Impl_Uint.ZERO, Make).
+
+  Definition tstore
+      (self : t)
+      (_address : Address.t)
+      (_index : aliases.U256.t)
+      (_value : aliases.U256.t) :
+      t :=
+    Make.
+
+  Definition log (self : t) (_log : Log.t LogData.t) : t :=
+    Make.
+
+  Definition selfdestruct
+      (self : t)
+      (_address : Address.t)
+      (_target : Address.t) :
+      option (StateLoad.t SelfDestructResult.t) * t :=
+    (None, Make).
+
   Instance I : Host.C t := {
+    Host.Cfg_t := t;
+    Host.Block_t := t;
+    Host.H_Cfg_t := IsLink;
+    Host.H_Block_t := IsLink;
+    Host.run_CfgGetter_for_Self := {|
+      Cfg.chain_id := chain_id;
+      Cfg.spec := spec;
+      Cfg.max_code_size := max_code_size;
+      Cfg.is_eip3607_disabled := is_eip3607_disabled;
+      Cfg.is_balance_check_disabled := is_balance_check_disabled;
+      Cfg.is_gas_refund_disabled := is_gas_refund_disabled;
+      Cfg.is_block_gas_limit_disabled := is_block_gas_limit_disabled;
+      Cfg.is_nonce_check_disabled := is_nonce_check_disabled;
+      Cfg.is_base_fee_check_disabled := is_base_fee_check_disabled;
+    |};
+    Host.run_Block_for_Block := {|
+      Block.number := number;
+      Block.beneficiary := beneficiary;
+      Block.timestamp := timestamp;
+      Block.gas_limit := gas_limit;
+      Block.basefee := basefee;
+      Block.difficulty := difficulty;
+      Block.prevrandao := prevrandao;
+      Block.blob_gasprice := blob_gasprice;
+    |};
+    Host.run_CfgGetter_for_Self := {| CfgGetter.cfg := cfg |};
+    Host.run_BlockGetter_for_Self := {| BlockGetter.block := block |};
     Host.load_account_delegated := load_account_delegated;
+    Host.block_hash := block_hash;
+    Host.balance := balance;
+    Host.code := code;
+    Host.code_hash := code_hash;
+    Host.sload := sload;
+    Host.sstore := sstore;
+    Host.tload := tload;
+    Host.tstore := tstore;
+    Host.log := log;
+    Host.selfdestruct := selfdestruct;
   }.
 End TestHost.
 Export (hints) TestHost.
@@ -33,6 +153,35 @@ Module TestHostWithAccount.
 
   Instance IsLink : Link t.
   Admitted.
+
+  Definition cfg : RefStub.t t t := {|
+    RefStub.path := [];
+    RefStub.projection self := self;
+    RefStub.injection _ y := y;
+  |}.
+  Definition block : RefStub.t t t := {|
+    RefStub.path := [];
+    RefStub.projection self := self;
+    RefStub.injection _ y := y;
+  |}.
+
+  Definition chain_id (_self : t) : u64 := {| Integer.value := 1 |}.
+  Definition spec (_self : t) : t := Make.
+  Definition max_code_size (_self : t) : usize := {| Integer.value := 0 |}.
+  Definition is_eip3607_disabled (_self : t) : bool := false.
+  Definition is_balance_check_disabled (_self : t) : bool := false.
+  Definition is_gas_refund_disabled (_self : t) : bool := false.
+  Definition is_block_gas_limit_disabled (_self : t) : bool := false.
+  Definition is_nonce_check_disabled (_self : t) : bool := false.
+  Definition is_base_fee_check_disabled (_self : t) : bool := false.
+  Definition number (_self : t) : u64 := {| Integer.value := 1 |}.
+  Definition beneficiary (_self : t) : Address.t := {| Address.value := 0 |}.
+  Definition timestamp (_self : t) : u64 := {| Integer.value := 0 |}.
+  Definition gas_limit (_self : t) : u64 := {| Integer.value := 0 |}.
+  Definition basefee (_self : t) : u64 := {| Integer.value := 0 |}.
+  Definition difficulty (_self : t) : aliases.U256.t := Impl_Uint.ZERO.
+  Definition prevrandao (_self : t) : option aliases.B256.t := None.
+  Definition blob_gasprice (_self : t) : option u128 := None.
 
   Definition test_account_load : AccountLoad.t := {|
     AccountLoad.load := {|
@@ -49,8 +198,95 @@ Module TestHostWithAccount.
       option AccountLoad.t * t :=
     (Some test_account_load, Make).
 
+  Definition block_hash (self : t) (_number : u64) :
+      option aliases.B256.t * t :=
+    (None, Make).
+
+  Definition balance (self : t) (_address : Address.t) :
+      option (StateLoad.t aliases.U256.t) * t :=
+    (None, Make).
+
+  Definition code (self : t) (_address : Address.t) :
+      option (Eip7702CodeLoad.t Bytes.t) * t :=
+    (None, Make).
+
+  Definition code_hash (self : t) (_address : Address.t) :
+      option (Eip7702CodeLoad.t aliases.B256.t) * t :=
+    (None, Make).
+
+  Definition sload (self : t) (_address : Address.t) (_index : aliases.U256.t) :
+      option (StateLoad.t aliases.U256.t) * t :=
+    (None, Make).
+
+  Definition sstore
+      (self : t)
+      (_address : Address.t)
+      (_index : aliases.U256.t)
+      (_value : aliases.U256.t) :
+      option (StateLoad.t SStoreResult.t) * t :=
+    (None, Make).
+
+  Definition tload (self : t) (_address : Address.t) (_index : aliases.U256.t) :
+      aliases.U256.t * t :=
+    (Impl_Uint.ZERO, Make).
+
+  Definition tstore
+      (self : t)
+      (_address : Address.t)
+      (_index : aliases.U256.t)
+      (_value : aliases.U256.t) :
+      t :=
+    Make.
+
+  Definition log (self : t) (_log : Log.t LogData.t) : t :=
+    Make.
+
+  Definition selfdestruct
+      (self : t)
+      (_address : Address.t)
+      (_target : Address.t) :
+      option (StateLoad.t SelfDestructResult.t) * t :=
+    (None, Make).
+
   Instance I : Host.C t := {
+    Host.Cfg_t := t;
+    Host.Block_t := t;
+    Host.H_Cfg_t := IsLink;
+    Host.H_Block_t := IsLink;
+    Host.run_CfgGetter_for_Self := {|
+      Cfg.chain_id := chain_id;
+      Cfg.spec := spec;
+      Cfg.max_code_size := max_code_size;
+      Cfg.is_eip3607_disabled := is_eip3607_disabled;
+      Cfg.is_balance_check_disabled := is_balance_check_disabled;
+      Cfg.is_gas_refund_disabled := is_gas_refund_disabled;
+      Cfg.is_block_gas_limit_disabled := is_block_gas_limit_disabled;
+      Cfg.is_nonce_check_disabled := is_nonce_check_disabled;
+      Cfg.is_base_fee_check_disabled := is_base_fee_check_disabled;
+    |};
+    Host.run_Block_for_Block := {|
+      Block.number := number;
+      Block.beneficiary := beneficiary;
+      Block.timestamp := timestamp;
+      Block.gas_limit := gas_limit;
+      Block.basefee := basefee;
+      Block.difficulty := difficulty;
+      Block.prevrandao := prevrandao;
+      Block.blob_gasprice := blob_gasprice;
+    |};
+    Host.run_CfgGetter_for_Self := {| CfgGetter.cfg := cfg |};
+    Host.run_BlockGetter_for_Self := {| BlockGetter.block := block |};
     Host.load_account_delegated := load_account_delegated;
+    Host.block_hash := block_hash;
+    Host.balance := balance;
+    Host.code := code;
+    Host.code_hash := code_hash;
+    Host.sload := sload;
+    Host.sstore := sstore;
+    Host.tload := tload;
+    Host.tstore := tstore;
+    Host.log := log;
+    Host.selfdestruct := selfdestruct;
   }.
 End TestHostWithAccount.
 Export (hints) TestHostWithAccount.
