RocqOfRust/core/simulate/default.v
@@ -1,0 +1,91 @@
+Require Import simulate.RocqOfRust.
+Require Import core.links.default.
+
+Module Default.
+  Class C (Self : Set) : Set := {
+    default : Self;
+  }.
+
+  Module Eq.
+    Class C
+        {Self : Set} `{Link Self}
+        `{!default.Default.Run Self}
+        `(!C Self) :
+        Prop := {
+      default (stack : Stack.t) :
+        {{
+          SimulateM.eval_f
+            (default.Default.run_default (Self := Self))
+            stack 🌲
+          (
+            Output.Success default,
+            stack
+          )
+        }};
+    }.
+  End Eq.
+  Export (hints) Eq.
+End Default.
+Export (hints) Default.
+
+Module Impl_Default_for_unit.
+  Definition Self : Set := unit.
+
+  Instance I : Default.C Self := {|
+    Default.default := tt;
+  |}.
+
+  Module Eq.
+    Instance I : Default.Eq.C (Self := Self) Impl_Default_for_unit.I.
+    Proof.
+      constructor; intros.
+      (* default *)
+      { s. }
+    Qed.
+  End Eq.
+  Export (hints) Eq.
+End Impl_Default_for_unit.
+Export (hints) Impl_Default_for_unit.
+
+Module Impl_Default_for_bool.
+  Definition Self : Set := bool.
+
+  Instance I : Default.C Self := {|
+    Default.default := false;
+  |}.
+
+  Module Eq.
+    Instance I : Default.Eq.C (Self := Self) Impl_Default_for_bool.I.
+    Proof.
+      constructor; intros.
+      (* default *)
+      { s. }
+    Qed.
+  End Eq.
+  Export (hints) Eq.
+End Impl_Default_for_bool.
+Export (hints) Impl_Default_for_bool.
+
+Module Impl_Default_for_integer.
+  Definition Self (kind : IntegerKind.t) : Set :=
+    Integer.t kind.
+
+  Definition default (kind : IntegerKind.t) : Self kind :=
+    {| Integer.value := 0 |}.
+
+  Instance I (kind : IntegerKind.t) : Default.C (Self kind) := {|
+    Default.default := default kind;
+  |}.
+
+  Module Eq.
+    Instance I (kind : IntegerKind.t) :
+      Default.Eq.C (Self := Self kind) (Impl_Default_for_integer.I kind).
+    Proof.
+      constructor; intros.
+      (* default *)
+      { destruct kind; s. }
+    Qed.
+  End Eq.
+  Export (hints) Eq.
+End Impl_Default_for_integer.
+Export (hints) Impl_Default_for_integer.
