RocqOfRust/revm/revm_context_interface/simulate/cfg.v
@@ -1,0 +1,187 @@
+Require Import simulate.RocqOfRust.
+Require Import revm.revm_context_interface.links.cfg.
+
+Module Cfg.
+  Class C
+      (Self : Set) `{Link Self}
+      (types : Cfg.Types.t) `{Cfg.Types.AreLinks types} :
+      Type := {
+    chain_id : Self -> u64;
+    spec : Self -> types.(Cfg.Types.Spec);
+    max_code_size : Self -> usize;
+    is_eip3607_disabled : Self -> bool;
+    is_balance_check_disabled : Self -> bool;
+    is_gas_refund_disabled : Self -> bool;
+    is_block_gas_limit_disabled : Self -> bool;
+    is_nonce_check_disabled : Self -> bool;
+    is_base_fee_check_disabled : Self -> bool;
+  }.
+
+  Module Eq.
+    Class t
+        {Self : Set} `{Link Self}
+        {types : Cfg.Types.t} `{Cfg.Types.AreLinks types}
+        (I : C Self types) :
+        Prop := {
+      chain_id
+          (stack : Stack.t)
+          (ref_self : '& Self)
+          (self : Self)
+          `{!Cfg.Method_chain_id Self} :
+        CanRead.t stack self ref_self ->
+        {{
+          SimulateM.eval_f
+            (Cfg.run_chain_id ref_self)
+            stack 🌲
+          (
+            Output.Success (I.(chain_id) self),
+            stack
+          )
+        }};
+      spec
+          (stack : Stack.t)
+          (ref_self : '& Self)
+          (self : Self)
+          `{!Cfg.Method_spec Self types} :
+        CanRead.t stack self ref_self ->
+        {{
+          SimulateM.eval_f
+            (Cfg.run_spec ref_self)
+            stack 🌲
+          (
+            Output.Success (I.(spec) self),
+            stack
+          )
+        }};
+      max_code_size
+          (stack : Stack.t)
+          (ref_self : '& Self)
+          (self : Self)
+          `{!Cfg.Method_max_code_size Self} :
+        CanRead.t stack self ref_self ->
+        {{
+          SimulateM.eval_f
+            (Cfg.run_max_code_size ref_self)
+            stack 🌲
+          (
+            Output.Success (I.(max_code_size) self),
+            stack
+          )
+        }};
+      is_eip3607_disabled
+          (stack : Stack.t)
+          (ref_self : '& Self)
+          (self : Self)
+          `{!Cfg.Method_is_eip3607_disabled Self} :
+        CanRead.t stack self ref_self ->
+        {{
+          SimulateM.eval_f
+            (Cfg.run_is_eip3607_disabled ref_self)
+            stack 🌲
+          (
+            Output.Success (I.(is_eip3607_disabled) self),
+            stack
+          )
+        }};
+      is_balance_check_disabled
+          (stack : Stack.t)
+          (ref_self : '& Self)
+          (self : Self)
+          `{!Cfg.Method_is_balance_check_disabled Self} :
+        CanRead.t stack self ref_self ->
+        {{
+          SimulateM.eval_f
+            (Cfg.run_is_balance_check_disabled ref_self)
+            stack 🌲
+          (
+            Output.Success (I.(is_balance_check_disabled) self),
+            stack
+          )
+        }};
+      is_block_gas_limit_disabled
+          (stack : Stack.t)
+          (ref_self : '& Self)
+          (self : Self)
+          `{!Cfg.Method_is_block_gas_limit_disabled Self} :
+        CanRead.t stack self ref_self ->
+        {{
+          SimulateM.eval_f
+            (Cfg.run_is_block_gas_limit_disabled ref_self)
+            stack 🌲
+          (
+            Output.Success (I.(is_block_gas_limit_disabled) self),
+            stack
+          )
+        }};
+      is_nonce_check_disabled
+          (stack : Stack.t)
+          (ref_self : '& Self)
+          (self : Self)
+          `{!Cfg.Method_is_nonce_check_disabled Self} :
+        CanRead.t stack self ref_self ->
+        {{
+          SimulateM.eval_f
+            (Cfg.run_is_nonce_check_disabled ref_self)
+            stack 🌲
+          (
+            Output.Success (I.(is_nonce_check_disabled) self),
+            stack
+          )
+        }};
+      is_base_fee_check_disabled
+          (stack : Stack.t)
+          (ref_self : '& Self)
+          (self : Self)
+          `{!Cfg.Method_is_base_fee_check_disabled Self} :
+        CanRead.t stack self ref_self ->
+        {{
+          SimulateM.eval_f
+            (Cfg.run_is_base_fee_check_disabled ref_self)
+            stack 🌲
+          (
+            Output.Success (I.(is_base_fee_check_disabled) self),
+            stack
+          )
+        }};
+    }.
+  End Eq.
+  Export (hints) Eq.
+End Cfg.
+Export (hints) Cfg.
+
+Module CfgGetter.
+  Class C
+      (Self : Set) `{Link Self}
+      (types : CfgGetter.Types.t)
+      `{CfgGetter.Types.AreLinks types} :
+      Type := {
+    Cfg_for_Cfg :: Cfg.C types.(CfgGetter.Types.Cfg) (CfgGetter.Types.to_Cfg_types types);
+    cfg : RefStub.t Self types.(CfgGetter.Types.Cfg);
+  }.
+
+  Module Eq.
+    Class t
+        {Self : Set} `{Link Self}
+        {types : CfgGetter.Types.t}
+        `{CfgGetter.Types.AreLinks types}
+        (I : C Self types) :
+        Prop := {
+      Cfg_for_Cfg :: Cfg.Eq.t I.(Cfg_for_Cfg);
+      cfg
+          (stack : Stack.t)
+          (ref_self : '& Self)
+          `{!CfgGetter.Method_cfg Self types} :
+        {{
+          SimulateM.eval_f
+            (CfgGetter.run_cfg ref_self)
+            stack 🌲
+          (
+            Output.Success (RefStub.apply ref_self I.(cfg)),
+            stack
+          )
+        }};
+    }.
+  End Eq.
+  Export (hints) Eq.
+End CfgGetter.
+Export (hints) CfgGetter.
